case_study/cc_lean/Definitions/Com.lean
@@ -75,36 +75,23 @@ inductive SmallStep : Com × State -> Com × State -> Prop where
   | while_loop (b c s) : SmallStep (WHILE b DO c, s) (IF b THEN c ;; WHILE b DO c ELSE SKIP, s)
 
 
-inductive RTC {α : Type} (R : α → α → Prop) (a : α) : α → Prop
-  | refl : RTC R a a
-  | tail (b c) (hab : RTC R a b) (hbc : R b c) : RTC R a c
+inductive RTC {α : Type} : (R : α → α → Prop) -> (a : α) -> (b : α) → Prop
+  | refl R a : RTC R a a
+  | step (b: α) c : (R a b -> RTC R b c ->  RTC R a c)
 
 
-theorem RTC_single {α : Type} {R : α → α → Prop} {a b : α} (hab : R a b) :
-    RTC R a b :=
-  RTC.tail _ _ RTC.refl hab
+theorem RTC_single {α : Type} {R : α → α → Prop} {a b : α} (hab : R a b) : RTC R a b := by
+  apply RTC.step
+  assumption
+  apply RTC.refl
 
-theorem RTC_lift {α β : Type} {R : α → α → Prop} {S : β → β → Prop} {a b : α}
-      (f : α → β) (hf : ∀a b, R a b → S (f a) (f b)) (hab : RTC R a b) :
-    RTC S (f a) (f b) :=
-  by
+theorem RTC_trans {α : Type} {R : α → α → Prop} {a b c : α} (hab : RTC R a b) (hbc : RTC R b c) : RTC R a c := by
     induction hab with
-    | refl => apply RTC.refl
-    | tail b c hab hbc ih =>
-      apply RTC.tail
-      apply ih
-      apply hf
-      exact hbc
-
-theorem RTC_trans {α : Type} {R : α → α → Prop} {a b c : α} (hab : RTC R a b)
-      (hbc : RTC R b c) :
-    RTC R a c :=
-  by
-    induction hbc with
-    | refl =>
-      assumption
-    | tail c d hbc hcd hac =>
-      apply RTC.tail <;>
+      | refl => assumption
+      | step _ _ _ _ ih => 
+        apply RTC.step
+        assumption
+        apply ih
         assumption
 
 --notation (name := small_step_judgement) init_config "->*" final_config => SmallStep init_config final_config
